Make progress towards removing fuel parameters from subparser functions

AllStar/Subparser.v
@@ -1,5 +1,5 @@
-Require Import Bool List String.
-Require Import Grammar Lib.Utils.
+Require Import Bool List Omega String.
+Require Import Grammar Lib.Utils Lib.Tactics.
 Import ListNotations.
 Open Scope string_scope.
 
@@ -11,56 +11,92 @@ Definition beqSp sp sp2 :=
   beqList sp.(stack) sp2.(stack) &&
   beqList sp.(prediction) sp2.(prediction).
 
-Definition moveSp (g : grammar)
-    (token : string) (sp : subparser) : list subparser :=
-  match sp.(stack) with
-  | nil => nil
-  | NT _ :: _ => [sp]
-  | T y :: stack' =>
-    if beqSym (T y) (T token) then
-      [mkSp stack' sp.(prediction)]
-    else
-      nil
-  end.
-
-Definition move (g : grammar) (sps : list subparser) (token : string) : list subparser :=
-  concat (map (moveSp g token) sps).
-
-Fixpoint spClosure (g    : grammar)
-                   (busy : list subparser)
-                   (fuel : nat)
-                   (sp   : subparser)
-                   : list subparser :=
-  match fuel with
-  | O => nil
-  | S n => 
-    if elem sp busy beqSp then
-      nil
-    else
+Definition move (token : string)
+                (sps   : list subparser) 
+                : list subparser :=
+  let moveSp sp := 
       match sp.(stack) with
       | nil => [sp]
-      | T _ :: _ => [sp]
-      | NT x :: stack' =>
-        let gammas := rhss g x in
-        let newSps :=
-            map (fun gamma =>
-                   mkSp (gamma ++ stack') sp.(prediction))
-                gammas
-        in concat (map (spClosure g (sp :: busy) n) newSps)
+      | NT _ :: _ => nil (* implementation error? *)
+      | T y :: stack' =>
+        if beqSym (T y) (T token) then 
+          [mkSp stack' sp.(prediction)] 
+        else 
+          nil
+      end 
+  in  concat (map moveSp sps).
+
+(* if removeOpt x l  = Some l', l' is a sublist of l *)
+Fixpoint removeOpt {A} (x : A) (l : list A) (beq : A -> A -> bool) :=
+  match l with
+  | nil => None
+  | y :: l' => 
+    if beq x y then
+      Some l'
+    else
+      match removeOpt x l' beq with
+      | None => None
+      | Some l'' => Some (y :: l'')
       end
   end.
 
-Definition closure (g : grammar) (sps : list subparser) :=
-  concat (map (spClosure g nil 100) sps).
+(* ... and here's the proof: *)
+Lemma removeOptDecreasing : forall A (x : A) beq (ys zs : list A),
+    removeOpt x ys beq = Some zs ->
+    List.length zs < List.length ys.
+Proof.
+  induction ys as [| y ys]; intros zs H.
+  - inversion H.
+  - simpl in H.
+    destruct (beq x y).
+    + inv H; simpl; omega.
+    + destruct (removeOpt x ys beq).
+      * inv H. simpl.
+        apply lt_n_S; apply IHys; reflexivity.
+      * inv H.
+Qed.
 
+(* Should be able to get rid of fuel because freeSyms is decreasing *)
+Fixpoint closure g freeSyms fuel sps :=
+  match fuel with 
+  | O => nil
+  | S n => concat (map (spClosure g freeSyms n) sps)
+  end
+with spClosure g freeSyms fuel sp :=
+       match fuel with 
+       | O => nil
+       | S n => 
+         match sp.(stack) with
+         | nil => [sp]
+         | T _ :: _ => [sp]
+         | NT x :: stack' => 
+           match removeOpt (NT x) freeSyms beqSym with
+           | None => nil (* recursion detected *)
+           | Some freeSyms' =>
+             let gammas := rhss g x in
+             let newSps := map (fun gamma => 
+                                  mkSp (gamma ++ stack') sp.(prediction)) gammas
+             in closure g freeSyms' n newSps
+           end
+         end
+       end.
+
+Definition nonterminals g :=
+  let prodNTs p :=
+      match p with
+      | (l, rs) => l :: filter isNT rs
+      end
+  in  concat (map prodNTs g).
+
+(* Remove fuel from the call to closure! *)
 Definition startState g x stack0 :=
   let gammas := rhss g x in
   let sps    := map (fun gamma =>
                        mkSp (gamma ++ stack0) gamma) gammas
-  in  closure g sps.
+  in  closure g (nonterminals g) 100 sps.
 
 Definition target g sps (token : string) :=
-  closure g (move g sps token ).
+  closure g (nonterminals g) 100 (move token sps).
 
 Fixpoint conflict sps : bool :=
   match sps with
